#+TITLE: PRA 99
#+DATE: <2019-05-15>
#+CATEGORIES: 专业笔记
#+TAGS: 物理, Cold Atoms, 散射
#+HTML: <!-- toc -->
#+HTML: <!-- more -->
* 

effective field theory , Hubbard-Stratonovich transformation
\begin{align}
  e^{-k^2/\bar{\Lambda}_s^2}
\end{align}
??
\begin{align}
  T_s(k \hat{k},k \hat{k}', E = \frac{k^2}{M}) 
  = - \frac{4 e^{-2k^2/ \bar{\Lambda}_s^2}}{V} D_s(\vec{q}=0 , E = \frac{k^2}{M})
\end{align}
$D_s$ 的系数是把相互作用摘出来?

[[file:./2019-05-15-专业笔记-PAR99/fig1.png]]

\begin{align}
  D = D_0 + D_0 \Sigma D
\end{align}

\begin{align}
  \frac{1}{D} = \frac{1}{D_0} - \Sigma
\end{align}

\begin{align}
  \frac{1}{D_0(\vec{q},E=\frac{k^2}{M})}
  = E - E_{\vec{q}} = \frac{k^2}{M} - \frac{1}{\bar{g}_s}
\end{align}

$\Sigma$ 先算零温, 再做解析延拓
\begin{align}
  \Sigma (\vec{q}, \mathrm{i}\Omega_m )
  =& \frac{1}{\beta}\sum_{n,\vec{k}}\frac{1}{\mathrm{i}\omega_n - E_{\frac{\vec{q}}{2}-\vec{k}}}
   \frac{1}{\mathrm{i}\Omega_m - \mathrm{i}\omega_n - E_{\frac{\vec{q}}{2}+\vec{k}}}\\
  =& \sum_{\vec{k}}
     \frac{1 +f(\frac{\vec{q}}{2} +\vec{k}) -f(\frac{\vec{q}}{2}-\vec{k})}
     {\mathrm{i}\Omega_m - E_{\frac{\vec{q}}{2}-\vec{k}} - E_{\frac{\vec{q}}{2} +\vec{k}} } \\
\end{align}
解析延拓
\begin{align}
  \Sigma (\vec{q}, E)
  =& \sum_{\vec{k}}
     \frac{1 +f(\frac{\vec{q}}{2} +\vec{k}) -f(\frac{\vec{q}}{2}-\vec{k})}
     {E - E_{\frac{\vec{q}}{2}-\vec{k}} - E_{\frac{\vec{q}}{2} +\vec{k}} +\mathrm{i}0^ +} \\
  =& \sum_{\vec{k}}
     \frac{1 +f(\frac{\vec{q}}{2} +\vec{k}) -f(\frac{\vec{q}}{2}-\vec{k})}
     {E - \frac{q^2}{4M}-\frac{k^2}{M} + \mathrm{i}0^ +} \\
\end{align}
若令 $f(\frac{\vec{q}}{2} +\vec{k}) =f(\frac{\vec{q}}{2}-\vec{k})=0$ ,
并且记 $\Omega = E -\frac{q^2}{4M}$ , 则
\begin{align}
  \Sigma (\vec{q}, \Omega) =& \sum_{\vec{k}}
     \frac{1}{\Omega-\frac{k^2}{M} + \mathrm{i}0^ +} \\
  =& -\mathrm{i}\frac{V}{4\pi}M\sqrt{M\Omega} -\sum_{\vec{k}}\frac{1}{k^2/M}
\end{align}
代回原式
\begin{align}
  \frac{1}{T_s(k \hat{k},k \hat{k}', E = \frac{k^2}{M})} 
  = - \frac{V}{4 e^{-2k^2/ \bar{\Lambda}_s^2}}
   \left[ \frac{k^2}{M} -\frac{1}{\bar{g}_s}
   +\mathrm{i}\frac{V}{4\pi}M\sqrt{ME} +\sum_{\vec{k}}\frac{M}{k^2} \right]
\end{align}
$s$ -wave phase shift (zeroth order of $k$)
\begin{align}
  \frac{1}{T_s(k \hat{k},k \hat{k}', E = \frac{k^2}{M})}
  =& -\frac{VM}{8\pi}\left(-\frac{1}{a_s} - \mathrm{i}k \right) \\
  =& \frac{VM}{8\pi}\frac{1}{a_s} + \mathrm{i}k\frac{VM}{8\pi}
\end{align}


* Reference 

PRA 99, 012701(2019)
