#+TITLE: Susskind's Particle Pyhsics Note
#+DATE: <2021-03-19>
#+CATEGORIES: 专业笔记
#+TAGS: physics, Particle Physics, Susskind, Quantum Field Theory, Stimulated Emission, Group Velocity, Phase Velocity
#+HTML: <!-- toc -->
#+HTML: <!-- more -->

* Information
- 官方介绍: https://theoreticalminimum.com/courses/particle-physics-1-basic-concepts/2009/fall

- 视频列表地址: https://www.youtube.com/watch?v=2eFvVzNF24g&list=PLaTmJYdn8i5zI1To7uSg75eNA_AKXGUl0

- 把主要内容整理一下.

* Lecture 1: Particles and Light

** Wave Properties

\begin{align}
\boxed{\frac{\lambda}{T} = c}
\end{align}
\begin{align}
f = \frac{1}{T} \quad \boxed{\lambda f = c}
\end{align}
\begin{align}
\omega = 2\pi f = \boxed{2\pi \frac{c}{\lambda} = \omega}
\end{align}

** Photon Properties

\begin{align}
\boxed{E_{\mathrm{phton}} = \hbar\omega}
\end{align}
\begin{align}
E_{\mathrm{ray}} = n \hbar \omega
\end{align}
\begin{align}
p = \frac{E}{c}
\end{align}

* Lecture 2: Review of Quantum Mechanics & Harmonic Oscillator

** Periodic Boundary Condition

In order to make momentum conseved, we need periodic boundary condition, so
\begin{align}
\lambda = \frac{L}{N}
\end{align}
$\lambda$ is discrete.
\begin{align}
p = \frac{h}{\lambda} = \frac{h}{L}N
\end{align}

** Harmonic Oscillator

\begin{align}
  E &= n \hbar\omega\\
  a^{+ }|n \rangle &= \sqrt{n + 1} | n+ 1 \rangle \\
  a^{- }|n \rangle &= \sqrt{n } | n - 1\rangle \\
  a^{+ }a^{- } &\sim n \\
  a^{- }a^{+ } &\sim n + 1
\end{align}

* Lecture 3: Field Operators

** Field operator

In periodic boundary conditions, a plane wave
\begin{align}
  e^{\mathrm{i}kL}, \quad, k = n\frac{2\pi}{L}
\end{align}
One particle with momentum $k_7$
\begin{align}
  |0, 0, 0, 0, 0, 0, 1, 0, 0, \cdots \rangle
\end{align}
Classical version of Fourier coefficient of field
\begin{align}
  \psi(x) &= \sum_k \alpha(k) e^{\mathrm{i} kx} \\
  \psi^{ * }(x) = \sum_k \alpha^{ * }(k) e^{- \mathrm{i}k x}
\end{align}
quantum version
\begin{align}
  \psi^{ -}(x) &= \sum_k \alpha^{- }(k) e^{\mathrm{i} kx} \\
  \psi^{ + }(x) &= \sum_k \alpha^{ + }(k) e^{- \mathrm{i}k x}
\end{align}
Let
\begin{align}
  |0\rangle \equiv& |0, 0, 0, 0, 0, 0\cdots \rangle\\
  |k_i\rangle \equiv& |0, 0, 0, \cdots , 1, 0, 0\cdots \rangle ,
    \quad\mathrm{one} \quad \mathrm{in}\quad i \mathrm{th}
\end{align}
Create a particle at position $x$
\begin{align}
  \psi^{+ }(x) |0\rangle = \sum_k e^{-\mathrm{i} k x} a^{+ }(k)| 0 \rangle
   = \sum_k e^{-\mathrm{i} k x} | k \rangle
\end{align}

** Possible  Reaction & Stimulated Emission

[[file:2021-03-19-专业笔记-SusskindsParticlePhysicsI/reaction.png]]

A particle comes in, and when it hits the target. The target happens to be
localized at position $x$ . That particle disappears. And then two particles
emitted from the same spot. How would we describe this reaction?
\begin{align}
  \Psi^{\dagger}(x) \Psi^{\dagger}(x) \Psi(x)|\rangle
\end{align}
If that a particle with momentum $k_i$ is absorbed at position $x$ . What is the
final state? What is the various probabilities for this final state to have this
or that momentum?

A photon comes in, hits an atom localized at a point and from that point two
photons go off
\begin{align}
  \Psi^{\dagger}(x) \Psi^{\dagger}(x) \Psi(x)|k_{\mathrm{i}}\rangle
  =& \sum_{l,m} a^{\dagger}(l) e^{-\mathrm{i}lx} a^{\dagger}(m) e^{-\mathrm{i}mx}
    \sum_k a(k) e^{\mathrm{i}kx} |k_{\mathrm{i}}\rangle \\
  =& \sum_{l,m} a^{\dagger}(l) e^{-\mathrm{i}lx} a^{\dagger}(m) e^{-\mathrm{i}mx}
      e^{\mathrm{i}k_{\mathrm{i}}x} |0\rangle \\
  =& \sum_{l,m} e^{\mathrm{i}(k_{\mathrm{i}} - l - m)}|l, m\rangle
\end{align}
本来想用这个说明 stimulated emission, 因为 $l = m$ 时会有 factor $\sqrt{2}$ ,
产生相同动量的两个粒子的概率会增加. 但是翻车了, 因为 $l \neq m$ 时, 同样也会有一个
$2$ , 因为 $l = 1, m = 2$ 和 $l = 2, m = 1$ 都会有贡献.

然后用另一个例子说明 stimulated emission. Supposing we have a particle which can
decay and emit a photon.
\begin{align}
  \Psi^{\dagger}(x) |0\rangle = \sum_k e^{-\mathrm{i} kx}|k\rangle
\end{align}
equal probability for all $k$ .

If there pre-exist a particle
\begin{align}
  \Psi^{\dagger}(x) |l\rangle = \sum_k e^{-\mathrm{i} kx} a^+(k)|l\rangle
\end{align}
if $k\neq l$
\begin{align}
  \Psi^{\dagger}(x) |l\rangle = \sum_k e^{-\mathrm{i} kx} |k, l\rangle
\end{align}
equal probability. But if $k = l$
\begin{align}
  e^{-\mathrm{i} kx} \sqrt{2}|k, k\rangle
\end{align}
There are no photons present then just decays with coefficient $1$ , that's
spontaneous emission. The presence of particles of a give type will increase the
probability that out decay takes places with the final momentum being the same
as the momentum already there. This is stimulated emission. Bosons!

** Density of $x$

\begin{align}
  \Psi^{\dagger}(x) \Psi(x)
\end{align}
\begin{align}
  \frac{1}{L}\int  \Psi^{\dagger}(x) \Psi(x) \cdot\mathrm{d}x = \frac{1}{L} = \mathrm{Number}
  \quad \mathrm{of} \quad \mathrm{particles}
\end{align}

* Lecture 4: Scattering Process

** Simplest Quantum Field

The simplest quantum field, be a function of only one coordinate namely $x$ .
\begin{align}
  \Psi (x, t) =& \sum_k a^-(k) e^{\mathrm{i}kx} e^{\mathrm{i}\omega(k)t}
   \quad \mathrm{(Definition)} \\
  \Psi^{\dagger} (x, t) =& \sum_k a^-(k) e^{-\mathrm{i}kx} e^{\mathrm{i}\omega(k)t}
\end{align}
Find the wave equation for $\Psi$ .
\begin{align}
  \frac{\partial}{\partial t} \Psi &= \mathrm{i} \omega(k) \Psi \\
  \frac{\partial}{\partial x} \Psi &= \mathrm{i} k \Psi \\
  \frac{\partial^2}{\partial x^2} \Psi &= - k^2 \Psi \\
\end{align}
so
\begin{align}
  \mathrm{i}\frac{\partial}{\partial t} \Psi = \frac{\omega}{k}\frac{\partial^2}{\partial x^2} \Psi
\end{align}
if $\omega = \frac{k^2}{2m}$ , a non-relativitic particle
\begin{align}
  \mathrm{i}\frac{\partial}{\partial t} \Psi = \frac{1}{2m}\frac{\partial^2}{\partial x^2} \Psi
\end{align}
$\Psi$ is an operator.

** A Model: Scattering

[[file:2021-03-19-专业笔记-SusskindsParticlePhysicsI/scattering.png]]

A particle absorbed by a fixed target and emitted by the target instantly. This
process is energy conserved but momentum not conserved. Averaging or integrating
over all possiable time (set $x_0 = 0$)
\begin{align}
 \langle k_f | g \int \mathrm{d}t\cdot \Psi^{\dagger}(0, t) \Psi(0, t) | k_i \rangle
  = 2 \pi g \delta (\omega_f - \omega_i)
\end{align}
where $g$ is coupling constant. There is connection between the fact that
conservation of eneryg and the fact there's no preference of any specified time.

* Lecture 5: Fermion

** Phase Velocity & Group Velocity

\begin{align}
\omega = \sqrt{k^2 + m^2}
\end{align}
for massless $m = 0$
\begin{align}
 v_{\mathrm{p}} &= \frac{\omega}{k} = 1 \\
 v_{\mathrm{g}} &= \frac{\mathrm{d}\omega}{\mathrm{d}k} = 1
\end{align}
but if $m \neq 0$
\begin{align}
 v_{\mathrm{p}} &= \frac{\omega}{k} = \sqrt{1 + \frac{m^2}{k^2}} > 1\\
 v_{\mathrm{g}} &= \frac{\mathrm{d}\omega}{\mathrm{d}k}
      = \sqrt{\frac{k^2}{k^2 + m^2}} < 1
\end{align}
$1$ is the speed of light. So phase velocity carries nothing.

** Fermion

\begin{align}
  c^{+ } |0 \rangle &= |1\rangle\\
  c^{+ } |1 \rangle &= 0\\
  c^{- } |0 \rangle &= 0\\
  c^{0 } |1 \rangle &= |0\rangle\\
\end{align}
\begin{align}
  \boxed{c^{+ } c^{ -} |0 \rangle  = 0 } \\
  \boxed{c^{- } c^{ +} |0 \rangle  = |0\rangle }
\end{align}

** Ground state

Boson: Bose condensate.

Fermion: Fermi sphere

** Dirac Equation

move speed of light( $\omega = k$ , $c = 1$ ), carry electric charge, only move to
one direction
filed $\Psi$
\begin{align}
  \Psi = e^{\mathrm{i}(k x - \omega t)} = e^{\mathrm{i} k (x - t)}
\end{align}
so
\begin{align}
  \frac{\partial \Psi}{\partial t} = - \frac{\partial \Psi}{\partial x}, \quad (\mathrm{i}\omega = \mathrm{i}k)
\end{align}
describe both positive and negative energy. Negative is filled.

* Lecture 6: Dirac Equation & Higgs Boson

Move right field
\begin{align}
   \frac{\partial \Psi}{\partial t} = - \frac{\partial \Psi}{\partial x}
\end{align}
Move left field
\begin{align}
  \frac{\partial \Psi}{\partial t} =  \frac{\partial \Psi}{\partial x} ,\quad (\omega = -k)
\end{align}
\begin{align}
  \dot{\Psi} \equiv \begin{pmatrix} \dot{\Psi}_R \\ \dot{\Psi}_L \end{pmatrix}
   = - \begin{pmatrix} 1 &0 \\0 & -1 \end{pmatrix}
    \begin{pmatrix} \frac{\partial \Psi_R}{\partial x} \\\frac{\partial \Psi_L}{\partial x} \end{pmatrix}
  \equiv - \alpha \frac{\partial}{\partial x} \Psi
\end{align}
\begin{align}
  \omega = \alpha k
\end{align}
we want (not massless) $\omega = \sqrt{k^2 + m^2}$ , so let $\omega = \alpha k + \beta m$
\begin{align}
  \omega^2 = k^2 + m^2 = (\alpha k + \beta m)^2 \Rightarrow \alpha^2 = 1, \beta^2 = 1, \alpha\beta + \beta\alpha = 0
\end{align}
so $\beta$ can be
\begin{align}
  \beta = \begin{pmatrix} 0 & 1 \\ 1 & 0 \end{pmatrix}
\end{align}
so
\begin{align}
  \mathrm{i} \begin{pmatrix} \dot{\Psi}_R \\ \dot{\Psi}_L \end{pmatrix}
  = - \mathrm{i} \alpha \frac{\partial}{\partial x}\Psi + \beta m \Psi
\end{align}
\begin{align}
  \mathrm{i}\dot{\Psi}_R =& -\mathrm{i}\partial_x \Psi_R + m\Psi_L \\
  \mathrm{i}\dot{\Psi}_L =& \mathrm{i}\partial_x \Psi_L + m\Psi_R
\end{align}
For a particle at rest ( $k = 0$ )
\begin{align}
  \mathrm{i} \frac{\partial}{\partial t} \Psi
   \equiv \mathrm{i} \begin{pmatrix} \dot{\Psi}_R \\\dot{\Psi}_L \end{pmatrix}= \beta m \Psi
   \equiv m \begin{pmatrix} \Psi_L \\ \Psi_R \end{pmatrix}
\end{align}

$\Psi_L$ and $\Psi_R$ are coupled. We can decouple them by $\Psi_+ = \Psi_L + \Psi_R$ ,
$\Psi_- = \Psi_L - \Psi_R$
\begin{align}
  \mathrm{i}\dot{\Psi}_+ &= m\Psi_+ \\
  \mathrm{i}\dot{\Psi}_- &= -m\Psi_-
\end{align}

** Dirac Equation in 3 Dimensions

Let
\begin{align}
  \omega =& \sqrt{k_1^2 + k_2^2 + k_3^2 + m^2} \\
  \omega =& \alpha k + \beta m = \alpha_1 k_1 + \alpha_2k_2 + \alpha_3 k_3 + \beta m
\end{align}
so
\begin{align}
\beta = \begin{pmatrix} I & 0 \\ 0 & -I \end{pmatrix}, \quad
\alpha_i   = \begin{pmatrix} 0 & \sigma_i \\ \sigma_i & 0 \end{pmatrix}
\end{align}
where $I$ is $2\times 2$ identity matrix, $\sigma_i$ is Pauli matrix.
\begin{align}
  \mathrm{i}\frac{\partial }{\partial t} \Psi_p = - i (\alpha_i)_{pq} \frac{\partial}{\partial x^i}\Psi_q
    + \beta_q m \Psi_q
\end{align}

* Lecture 7: Angular Momentum

Angular momentum
- Orbital
- Spin

\begin{align}
  [x_i , x_j] &= 0 \\
  [p_i , p_j] &= 0 \\
  [x, p_x] &= \mathrm{i}\hbar \\
  [x_i, p_j] &= \mathrm{i}\hbar\delta_{ij} \\
  [L_x, L_y] &= \mathrm{i}\hbar L_z
\end{align}
\begin{align}
  L_+ &= L_x + \mathrm{i} L_y \\
  L_- &= L_x - \mathrm{i} L_y \\
\end{align}
\begin{align}
  [L_{+} , L_z] &= - L_{ +} \\
  [L_{- }, L_z] &= + L_-
\end{align}

* Lecture 8: Spin

Review spin.

* Lecture 9: Interaction

Diagrams but abstract.

* Lecture 10: Path Integral

Abstract.

* Reference
